run.sh
@@ -3,5 +3,5 @@
 # AVL.fst BinTree.fst BDD.fst MapAVL.fst SetAVL.fst Compare.fst
 fstar.exe --record_hints --use_hints --odir fstar_out --codegen OCaml BDD.fst --query_stats 
 cd fstar_out 
-# ocamlbuild BDD2.native -package fstarlib,batteries
+ocamlbuild BDD.native -package fstarlib,batteries
 cd ..
